Common/CMaps.v
@@ -481,6 +481,15 @@ Section DMap.
     apply proof_irrelevance.
   Qed.
 
+  #[global] Instance dmap_eq_dec `{EqDecision (sigT F)} :
+      EqDecision dmap.
+  Proof.
+    intros m m'.
+    destruct (decide (dmap_car m = dmap_car m')) as [Heq | Hneq].
+    - left. apply dmap_eq_car. exact Heq.
+    - right. intros Heq. apply Hneq. congruence.
+  Defined.
+
   Lemma dmap_eq m m': (∀ k : K, m !d! k = m' !d! k) → m = m'.
   Proof using ctrans_F_simpl.
     intro H.
