Common/CExtraction.v
@@ -56,6 +56,8 @@ Extract Inlined Constant Decision => "bool".
 Extract Inlined Constant Bool.eqb => "(=)".
 Extraction Inline decide.
 Extraction Inline decide_rel.
+Extract Inlined Constant Exec.runtime_hash =>
+  "(fun x -> ZO.succ (ZO.of_int (Hashtbl.hash x)))".
 
 (** * Integers
 
